Add #8 solution

tasks/008/Solution.v
@@ -1,5 +1,411 @@
-Require Import Problem PeanoNat List Omega.
+Require Import Problem PeanoNat List Omega Permutation.
+Import ListNotations.
+
+Fixpoint sorted (xs : list nat) :=
+  match xs with
+  | nil => True
+  | x :: ys =>
+    match ys with
+    | nil => True
+    | y :: zs => x <= y /\ sorted ys
+    end
+  end.
+
+Definition all (P : nat -> Prop) (xs : list nat) := fold_right and True (map P xs).
+Definition upper_bound (n : nat) := all (fun x => x <= n).
+Definition lower_bound (n : nat) := all (fun x => n <= x).
+
+Lemma perm_dig : forall x xs ys, Permutation (A:=nat) (x :: xs) ys -> exists zs ws, ys = zs ++ x :: ws.
+Proof.
+  intros.
+  assert (In x ys) by (refine (Permutation_in _ H _); simpl; auto); clear H.
+  induction ys; [inversion H0|].
+  simpl in H0.
+  destruct H0; [subst a; exists nil; exists ys; auto|].
+  apply IHys in H; clear IHys.
+  destruct H; destruct H.
+  exists (a :: x0); exists x1.
+  subst ys.
+  auto.
+Qed.
+
+Lemma perm_all : forall P xs, all P xs -> forall ys, Permutation xs ys -> all P ys.
+Proof.
+  induction xs; intros.
+  - apply Permutation_nil in H0.
+    subst ys; simpl; auto.
+  - unfold all in H; simpl in H; fold (all P xs) in H.
+    destruct H.
+    specialize (IHxs H1); clear H1.
+    destruct (perm_dig a xs ys H0); destruct H1.
+    subst ys.
+    assert (Permutation (a :: x ++ x0) (x ++ a :: x0)) by apply Permutation_middle.
+    apply Permutation_sym in H1.
+    assert (Permutation (a :: xs) (a :: x ++ x0)).
+    * apply (Permutation_trans H0 H1); clear H1.
+    * apply Permutation_cons_inv in H2.
+      apply IHxs in H2.
+      clear IHxs H1 H0.
+      induction x.
+      + unfold all; simpl; fold (all P x0).
+        simpl in H2.
+        auto.
+      + unfold all; simpl; fold (all P (x ++ a :: x0)).
+        unfold all in H2; simpl in H2; fold (all P (x ++ x0)) in H2.
+        destruct H2.
+        auto.
+Qed.
+
+Lemma perm_upper : forall n xs, upper_bound n xs -> forall ys, Permutation xs ys -> upper_bound n ys.
+Proof.
+  intro.
+  unfold upper_bound.
+  apply (perm_all (fun x => x <= n)).
+Qed.
+
+Lemma perm_lower : forall n xs, lower_bound n xs -> forall ys, Permutation xs ys -> lower_bound n ys.
+Proof.
+  intro.
+  unfold lower_bound.
+  apply (perm_all (fun x => n <= x)).
+Qed.
+
+Lemma sorted_app : forall xs n ys, upper_bound n xs -> lower_bound n ys -> sorted xs -> sorted ys -> sorted (xs ++ [n] ++ ys).
+Proof.
+  intros.
+  induction xs; simpl.
+  - destruct ys; [auto|].
+    destruct H0; split; auto.
+  - destruct H.
+    destruct xs.
+    * simpl.
+      clear H3 H1; simpl in IHxs; specialize (IHxs I I).
+      split; auto.
+    * simpl; simpl in IHxs; simpl in H1.
+      destruct H1.
+      split; [auto|].
+      fold (all (fun x : nat => x <= n) (n0 :: xs)) in H3.
+      fold (upper_bound n (n0 :: xs)) in H3.
+      apply IHxs; auto.
+Qed.
+
+Lemma filter_short (P : nat -> bool) : forall xs, length (filter P xs) <= length xs.
+Proof.
+  induction xs; simpl; [auto|].
+  destruct (P a); simpl; omega.
+Qed.
+
+Lemma move_to_left (x :nat) (ys zs : list nat) : Permutation (x :: ys ++ zs) (ys ++ x :: zs).
+Proof.
+  replace (x :: ys ++ zs) with (([x] ++ ys) ++ zs) by auto.
+  replace (ys ++ x :: zs) with ((ys ++ [x]) ++ zs) by (rewrite <- app_assoc; auto).
+  apply Permutation_app_tail.
+  apply Permutation_app_comm.
+Qed.
+
+Lemma filter_split (P Q : nat -> bool) : (forall x, P x = negb (Q x)) -> forall xs, Permutation xs (filter P xs ++ filter Q xs).
+Proof.
+  intros.
+  induction xs; simpl; [constructor|].
+  specialize (H a).
+  destruct (Q a); rewrite H; simpl; [|apply perm_skip; auto].
+  apply (perm_skip a) in IHxs.
+  refine (Permutation_trans IHxs _).
+  apply Permutation_middle.
+Qed.
+
+Definition lt_n (n : nat) := fun x => x <? n.
+Definition ge_n (n : nat) := fun x => n <=? x.
+Definition le_n (n : nat) := fun x => x <=? n.
+Definition gt_n (n : nat) := fun x => n <? x.
+
+Lemma lt_upper : forall n xs, upper_bound n (filter (lt_n n) xs).
+Proof.
+  unfold upper_bound; unfold all.
+  induction xs; simpl; [auto|].
+  unfold lt_n.
+  assert (a < n \/ a >= n) by omega.
+  destruct H.
+  assert (a <? n = true) by (apply Nat.ltb_lt; auto).
+  rewrite H0.
+  simpl.
+  split; [omega|auto].
+  apply Nat.ltb_ge in H.
+  rewrite H.
+  auto.
+Qed.
+
+Lemma le_upper : forall n xs, upper_bound n (filter (le_n n) xs).
+Proof.
+  unfold upper_bound; unfold all.
+  induction xs; simpl; [auto|].
+  unfold le_n.
+  assert (a <= n \/ a > n) by omega.
+  destruct H.
+  assert (a <=? n = true) by (apply Nat.leb_le; auto).
+  rewrite H0.
+  simpl.
+  split; [omega|auto].
+  apply Nat.leb_gt in H.
+  rewrite H.
+  auto.
+Qed.
+
+Lemma ge_lower : forall n xs, lower_bound n (filter (ge_n n) xs).
+Proof.
+  unfold lower_bound; unfold all.
+  induction xs; simpl; [auto|].
+  unfold ge_n.
+  assert (n <= a \/ n > a) by omega.
+  destruct H.
+  assert (n <=? a = true) by (apply Nat.leb_le; auto).
+  rewrite H0.
+  simpl.
+  split; [omega|auto].
+  apply Nat.leb_gt in H.
+  rewrite H.
+  auto.
+Qed.
+
+Lemma gt_lower : forall n xs, lower_bound n (filter (gt_n n) xs).
+Proof.
+  unfold lower_bound; unfold all.
+  induction xs; simpl; [auto|].
+  unfold gt_n.
+  assert (n < a \/ n >= a) by omega.
+  destruct H.
+  assert (n <? a = true) by (apply Nat.ltb_lt; auto).
+  rewrite H0.
+  simpl.
+  split; [omega|auto].
+  apply Nat.ltb_ge in H.
+  rewrite H.
+  auto.
+Qed.
+
+Lemma sort_mid : forall x ys z ws, sorted (x :: ys ++ z :: ws) -> x <= z.
+Proof.
+  induction ys; simpl; intros.
+  destruct H; auto.
+  destruct H.
+  destruct ys.
+  simpl in H0; simpl in IHys.
+  destruct H0.
+  omega.
+  simpl in IHys.
+  simpl in H0.
+  apply (IHys z ws).
+  destruct H0.
+  split; [omega|auto].
+Qed.
+
+Lemma qs1_split : forall n xs, Permutation xs (filter (lt_n n) xs ++ filter (ge_n n) xs).
+Proof.
+  intros.
+  apply filter_split.
+  intros.
+  unfold lt_n; unfold ge_n.
+  apply Nat.ltb_antisym.
+Qed.
+
+Lemma qs2_split : forall n xs, Permutation xs (filter (le_n n) xs ++ filter (gt_n n) xs).
+Proof.
+  intros.
+  apply filter_split.
+  intros.
+  unfold le_n; unfold gt_n.
+  apply Nat.leb_antisym.
+Qed.
+
+Lemma qs1_perm : forall xs ys, quicksort1 xs ys -> Permutation xs ys.
+Proof.
+  intro.
+  remember (length xs) as k.
+  assert (length xs <= k) by omega; clear Heqk.
+  revert xs H.
+  induction k; intros.
+  - apply Nat.le_0_r in H.
+    apply length_zero_iff_nil in H.
+    subst xs.
+    inversion H0; constructor.
+  - destruct xs; [inversion H0; constructor|].
+    simpl in H.
+    assert (length xs <= k) by omega; clear H.
+    inversion H0; clear H0.
+    subst head tail ys.
+    refine (Permutation_trans _ (move_to_left n l r)).
+    apply perm_skip.
+    fold (lt_n n) in H3; fold (ge_n n) in H5.
+    refine (Permutation_trans (qs1_split n xs) _).
+    remember (filter (lt_n n) xs) as xs_l.
+    remember (filter (ge_n n) xs) as xs_r.
+    refine (Permutation_app _ _); (apply IHk; [|auto]).
+    assert (length xs_l <= length xs) by (subst xs_l; apply filter_short); omega.
+    assert (length xs_r <= length xs) by (subst xs_r; apply filter_short); omega.
+Qed.
+
+
+Lemma qs2_perm : forall xs ys, quicksort2 xs ys -> Permutation xs ys.
+Proof.
+  intro.
+  remember (length xs) as k.
+  assert (length xs <= k) by omega; clear Heqk.
+  revert xs H.
+  induction k; intros.
+  - apply Nat.le_0_r in H.
+    apply length_zero_iff_nil in H.
+    subst xs.
+    inversion H0; constructor.
+  - destruct xs; [inversion H0; constructor|].
+    simpl in H.
+    assert (length xs <= k) by omega; clear H.
+    inversion H0; clear H0.
+    subst head tail ys.
+    refine (Permutation_trans _ (move_to_left n l r)).
+    apply perm_skip.
+    fold (le_n n) in H3; fold (gt_n n) in H5.
+    refine (Permutation_trans (qs2_split n xs) _).
+    remember (filter (le_n n) xs) as xs_l.
+    remember (filter (gt_n n) xs) as xs_r.
+    refine (Permutation_app _ _); (apply IHk; [|auto]).
+    assert (length xs_l <= length xs) by (subst xs_l; apply filter_short); omega.
+    assert (length xs_r <= length xs) by (subst xs_r; apply filter_short); omega.
+Qed.
+
+Lemma qs1_sorted : forall xs ys, quicksort1 xs ys -> sorted ys.
+Proof.
+  intro.
+  remember (length xs) as k.
+  assert (length xs <= k) by omega; clear Heqk.
+  revert xs H.
+  induction k; intros.
+  apply Nat.le_0_r in H.
+  apply length_zero_iff_nil in H.
+  subst xs; inversion H0; simpl; auto.
+  destruct xs; [inversion H0; simpl; auto|].
+  simpl in H; assert (length xs <= k) by omega; clear H.
+  inversion H0; clear H0.
+  subst head tail ys.
+  fold (lt_n n) in H3; fold (ge_n n) in H5.
+  remember (filter (lt_n n) xs) as xs_l.
+  remember (filter (ge_n n) xs) as xs_r.
+  apply sorted_app.
+  apply qs1_perm in H3.
+  apply (perm_upper n xs_l); [|auto].
+  subst xs_l; apply lt_upper.
+  apply qs1_perm in H5.
+  apply (perm_lower n xs_r); [|auto].
+  subst xs_r; apply ge_lower.
+  apply (IHk xs_l); [|auto].
+  assert (length xs_l <= length xs) by (subst xs_l; apply filter_short); omega.
+  apply (IHk xs_r); [|auto].
+  assert (length xs_r <= length xs) by (subst xs_r; apply filter_short); omega.
+Qed.
+
+Lemma qs2_sorted : forall xs ys, quicksort2 xs ys -> sorted ys.
+Proof.
+  intro.
+  remember (length xs) as k.
+  assert (length xs <= k) by omega; clear Heqk.
+  revert xs H.
+  induction k; intros.
+  apply Nat.le_0_r in H.
+  apply length_zero_iff_nil in H.
+  subst xs; inversion H0; simpl; auto.
+  destruct xs; [inversion H0; simpl; auto|].
+  simpl in H; assert (length xs <= k) by omega; clear H.
+  inversion H0; clear H0.
+  subst head tail ys.
+  fold (le_n n) in H3; fold (gt_n n) in H5.
+  remember (filter (le_n n) xs) as xs_l.
+  remember (filter (gt_n n) xs) as xs_r.
+  apply sorted_app.
+  apply qs2_perm in H3.
+  apply (perm_upper n xs_l); [|auto].
+  subst xs_l; apply le_upper.
+  apply qs2_perm in H5.
+  apply (perm_lower n xs_r); [|auto].
+  subst xs_r; apply gt_lower.
+  apply (IHk xs_l); [|auto].
+  assert (length xs_l <= length xs) by (subst xs_l; apply filter_short); omega.
+  apply (IHk xs_r); [|auto].
+  assert (length xs_r <= length xs) by (subst xs_r; apply filter_short); omega.
+Qed.
+
+Lemma sort_uniq : forall xs ys, Permutation xs ys -> sorted xs -> sorted ys -> xs = ys.
+Proof.
+  induction xs; simpl; intros.
+  apply Permutation_nil in H.
+  auto.
+  assert (lower_bound a (a :: xs)).
+  clear H IHxs H1 ys.
+  unfold lower_bound; unfold all.
+  simpl; split; [omega|].
+  induction xs.
+  auto.
+  simpl.
+  destruct H0.
+  split; [auto|].
+  apply IHxs; clear IHxs.
+  destruct xs; [auto|].
+  destruct H0.
+  split; [omega|auto].
+
+  assert (lower_bound a ys).
+  refine (perm_lower _ _ H2 _ H).
+  clear H2.
+
+  destruct (perm_dig a _ _ H); destruct H2.
+  subst ys.
+  destruct x.
+  simpl.
+  f_equal.
+  apply IHxs.
+  simpl in H.
+  apply Permutation_cons_inv in H.
+  auto.
+  destruct xs.
+  auto.
+  destruct H0.
+  auto.
+  simpl in H1.
+  destruct x0.
+  auto.
+  destruct H1.
+  auto.
+
+  assert (a <= n).
+  unfold lower_bound in H3; unfold all in H3; destruct H3; auto.
+  rewrite <- app_comm_cons in H1.
+  assert (n <= a) by (apply sort_mid in H1; auto).
+  assert (n = a) by omega; clear H2 H4.
+  subst n.
+  simpl.
+  f_equal.
+  apply IHxs.
+  simpl in H.
+  apply Permutation_cons_inv in H; auto.
+  destruct xs.
+  auto.
+  destruct H0.
+  auto.
+  remember (x ++ a :: x0) as t.
+  simpl in H1.
+  destruct t.
+  auto.
+  destruct H1.
+  auto.
+Qed.
 
 Theorem solution : task.
 Proof.
-Admitted.
+  unfold task.
+  intros.
+  apply sort_uniq.
+  - apply qs1_perm in H.
+    apply qs2_perm in H0.
+    apply Permutation_sym in H.
+    apply (Permutation_trans H H0).
+  - apply qs1_sorted in H; auto.
+  - apply qs2_sorted in H0; auto.
+Qed.
